tweaking lib

src/lib/GPU.fsti
@@ -15,18 +15,9 @@ include GPU.Array
 include GPU.Kernel
 include GPU.SizeT
 include GPU.Conditional
+include GPU.IntAliases
+include GPU.AtomicOps
 
-include GPU.Float32 { float }
-include GPU.Float64 { double }
+include Pulse.Lib.GhostReference { ref as gref, pts_to as gref_pts_to }
 
-unfold type f32 = float
-unfold type f64 = double
-unfold type u8  = FStar.UInt8.t
-unfold type u16 = FStar.UInt16.t
-unfold type u32 = FStar.UInt32.t
-unfold type u64 = FStar.UInt64.t
-unfold type i8  = FStar.Int8.t
-unfold type i16 = FStar.Int16.t
-unfold type i32 = FStar.Int32.t
-unfold type i64 = FStar.Int64.t
-unfold type sz  = FStar.SizeT.t
+include GPU.Seq.Common { op_At_Bang }
