src/lib/GPU.IntAliases.fsti
@@ -1,0 +1,16 @@
+module GPU.IntAliases
+
+include GPU.Float32 { float }
+include GPU.Float64 { double }
+
+unfold type f32 = float
+unfold type f64 = double
+unfold type u8  = FStar.UInt8.t
+unfold type u16 = FStar.UInt16.t
+unfold type u32 = FStar.UInt32.t
+unfold type u64 = FStar.UInt64.t
+unfold type i8  = FStar.Int8.t
+unfold type i16 = FStar.Int16.t
+unfold type i32 = FStar.Int32.t
+unfold type i64 = FStar.Int64.t
+unfold type sz  = FStar.SizeT.t
