src/lib/GPU.Seq.Common.fsti
@@ -1,0 +1,16 @@
+module GPU.Seq.Common
+
+open FStar.Seq
+
+unfold
+let ( @! ) (#a:Type) (s : seq a) (i : nat { i < Seq.length s }) : a = Seq.index #a s i
+
+let rec seq_fold_left (#t:Type) (f: t -> t -> t) (acc: t) (v: seq t)
+: Tot t (decreases length v)
+=
+  if length v = 0 then
+    acc
+  else
+    let hd = head v in
+    let tl = tail v in
+    seq_fold_left f (f acc hd) tl
